\documentclass[10pt]{article}
\usepackage{amsmath}

\begin{document}
The \textit{symmetrically recursive} kernel $Q_d:\mathbf{C}^{2^d}\to\mathbf{C}^{2^d}$ is a linear isometry, defined recursively by $Q_0=\left(1\right)$ and

\[
Q_{d+1}=\frac{1}{\sqrt{2}}
\left(
\begin{matrix}
\prod_{i=1}^d C_{d,i} Q_d & \prod_{i=1}^d C_{d,i} Q_d \\
\prod_{i=1}^d D_{d,i} Q_d & -\prod_{i=1}^d D_{d,i} Q_d
\end{matrix}\right)
\]

$D_{d,i}(0),\dots,D_{d,i}(2^d-1)$ and $C_{d,i}(0),\dots,C_{d,i}(2^d-1)$ are sequences of independent equiprobable $\{+1,-1\}$ random variables in:
\[
D_{d,i} = \left(
\begin{matrix}
D_{d,i}(0) & \dots & 0 \\
\vdots & \ddots & \vdots \\
0 & \dots & D_{d,i}(2^d-1)
\end{matrix}\right)
\quad
C_{d,i} = \left(
\begin{matrix}
C_{d,i}(0) & \dots & 0 \\
\vdots & \ddots & \vdots \\
0 & \dots & C_{d,i}(2^d-1)
\end{matrix}\right)
\]

We aim to derive a polynomial expression for $y^{d+1}_j=(Q_{d+1}x)_j$, where $x\in\mathbf{C}^{2^{d+1}}$ is comprised of the elements $x(b_0,\dots, b_{d})\in\mathbf{C}$ for $b_i\in\{0,1\}$.

$y^{d+1}_j$ is a polynomial in:
\begin{enumerate}
	\item $x(b_0,\dots, b_{d})$, for all $b_i\in\{0,1\}$
	\item $C_{p,i}$ and $D_{p,i}$, for all $0\le p<d+1$ and $1\le i < p$
\end{enumerate}

The base case is $y_0^0=Q_0x=x_0$.

\end{document}
